Needs "refines" invariant

Correctness.thy
@@ -19,21 +19,45 @@ case False with reds_avoids_live[OF assms(1,2)]
   thus ?thesis by simp
 qed
 
+inductive refines where
+  refinesI: "(\<And> x e. (x, e) \<in> set \<Gamma> \<Longrightarrow> x \<in> fdom \<rho> \<Longrightarrow> the (lookup \<rho> x) \<sqsubseteq> \<lbrakk>e\<rbrakk>\<^bsub>fmap_expand \<rho> (fdom \<rho> \<union> fst `set \<Gamma>)\<^esub>) \<Longrightarrow> refines \<Gamma> \<rho>"
+
+lemma refinesD:
+  assumes "refines \<Gamma> \<rho>"
+  assumes "(x, e) \<in> set \<Gamma>"
+  assumes "x \<in> fdom \<rho>"
+  shows "the (lookup \<rho> x) \<sqsubseteq> \<lbrakk>e\<rbrakk>\<^bsub>fmap_expand \<rho> (fdom \<rho> \<union> fst `set \<Gamma>)\<^esub>"
+using assms by (metis refines.simps)
+
+lemma refinesD':
+  assumes "refines \<Gamma> \<rho>"
+  assumes "(x, e) \<in> set \<Gamma>"
+  assumes "x \<in> fdom \<rho> \<union> fst ` set \<Gamma>"
+  shows "the (lookup (fmap_expand \<rho> (fdom \<rho> \<union> fst `set \<Gamma>)) x) \<sqsubseteq> \<lbrakk>e\<rbrakk>\<^bsub>fmap_expand \<rho> (fdom \<rho> \<union> fst `set \<Gamma>)\<^esub>"
+  using assms
+  apply (cases "x \<in> fdom \<rho>")
+  apply (auto dest: refinesD)
+  done
+
+
 theorem correctness:
-  assumes "\<Gamma> : e \<Down>\<^bsub>L\<^esub> \<Delta> : z"
-  shows "\<lbrakk>e\<rbrakk>\<^bsub>\<lbrace>\<Gamma>\<rbrace>\<rho>\<^esub> = \<lbrakk>z\<rbrakk>\<^bsub>\<lbrace>\<Delta>\<rbrace>\<rho>\<^esub>" and "\<lbrace>\<Gamma>\<rbrace>\<rho> \<le> \<lbrace>\<Delta>\<rbrace>\<rho>"
+  assumes "\<Gamma> : e \<Down>\<^bsub>L\<^esub> \<Delta> : z" and "refines \<Gamma> \<rho>"
+  shows "\<lbrakk>e\<rbrakk>\<^bsub>\<lbrace>\<Gamma>\<rbrace>\<rho>\<^esub> = \<lbrakk>z\<rbrakk>\<^bsub>\<lbrace>\<Delta>\<rbrace>\<rho>\<^esub>" and "\<lbrace>\<Gamma>\<rbrace>\<rho> \<le> \<lbrace>\<Delta>\<rbrace>\<rho>" and "refines \<Delta> \<rho>"
   using assms
 proof(nominal_induct avoiding: \<rho>  rule:reds.strong_induct)
 print_cases
-case Lambda
+case (Lambda \<Gamma> x e L \<rho>)
   print_cases
   case 1 show ?case by simp
   case 2 show ?case by simp
+  case 3 show ?case by fact
 next
 
 case (Application y \<Gamma> e x L \<Delta> \<Theta> z e' \<rho>)
 
   case 1
+  note Application.hyps(10,11,12)[OF `refines \<Gamma> \<rho>`]
+  note Application.hyps(14,15,16)[OF `refines \<Delta> \<rho>`]
   have "\<lbrakk> App e x \<rbrakk>\<^bsub>\<lbrace>\<Gamma>\<rbrace>\<rho>\<^esub> = \<lbrakk> e \<rbrakk>\<^bsub>\<lbrace>\<Gamma>\<rbrace>\<rho>\<^esub> \<down>Fn \<lbrakk> Var x \<rbrakk>\<^bsub>\<lbrace>\<Gamma>\<rbrace>\<rho>\<^esub>"
     by simp also
   have "... = \<lbrakk> Lam [y]. e' \<rbrakk>\<^bsub>\<lbrace>\<Delta>\<rbrace>\<rho>\<^esub> \<down>Fn \<lbrakk> Var x \<rbrakk>\<^bsub>\<lbrace>\<Gamma>\<rbrace>\<rho>\<^esub>"
@@ -52,45 +76,72 @@ case (Application y \<Gamma> e x L \<Delta> \<Theta> z e' \<rho>)
   finally
   show ?case .
   case 2 show ?case using `\<lbrace>\<Gamma>\<rbrace>\<rho> \<le> _` `\<lbrace>\<Delta>\<rbrace>\<rho> \<le> _`  by simp
+  case 3 show ?case by fact
 next
 
 case (Variable x e \<Gamma> L \<Delta> z \<rho>)
   have xnot1: "x \<notin> fst ` set (removeAll (x, e) \<Gamma>)" sorry
   have xnot2: "x \<notin> fst ` set \<Delta>" sorry
 
+  have cond: "heapExtendJoin_cond' ((x, e) # removeAll (x, e) \<Gamma>) ESem \<rho>" sorry
+  have cond2: "heapExtendJoin_cond' ((x, z) # \<Delta>) ESem \<rho>" sorry
+
+  let "?S" = "(fix_join_compat'' (fmap_expand \<rho> (fdom \<rho> \<union> fst ` set ((x, e) # removeAll (x, e) \<Gamma>)))
+       (\<lambda>\<rho>'a. fmap_expand (heapToEnv ((x, e) # removeAll (x, e) \<Gamma>) (\<lambda>e. \<lbrakk> e \<rbrakk>\<^bsub>\<rho>'a\<^esub>))
+               (fdom \<rho> \<union> fst ` set ((x, e) # removeAll (x, e) \<Gamma>))))"
+  let "?S2" = "(fix_join_compat'' (fmap_expand \<rho> (fdom \<rho> \<union> fst ` set ((x, z) # \<Delta>)))
+       (\<lambda>\<rho>'a. fmap_expand (heapToEnv ((x, z) # \<Delta>) (\<lambda>e. \<lbrakk> e \<rbrakk>\<^bsub>\<rho>'a\<^esub>))
+               (fdom \<rho> \<union> fst ` set ((x, z) # \<Delta>))))"
+
   case 2
   have "\<lbrace>\<Gamma>\<rbrace>\<rho> = \<lbrace>(x,e) # removeAll (x,e) \<Gamma>\<rbrace>\<rho>" sorry also (* Distinctness and reordering lemma needed *)
-  have "... = fix1 (fmap_bottom (fdom \<rho> \<union> fst ` set ((x, e) # removeAll (x, e) \<Gamma>)))
-                   (\<Lambda> \<rho>'a. fmap_update \<rho>
-                            (fmap_restr (fst ` set (removeAll (x, e) \<Gamma>)) (\<lbrace>removeAll (x, e) \<Gamma>\<rbrace>\<rho>'a)(x f\<mapsto> \<lbrakk> e \<rbrakk>\<^bsub>\<rho>'a\<^esub>)))"                           
-    by (rule iterative_HSem[OF _ xnot1]) also (* Alternative definition needs to be proven *)
-  have "... = fix1 (fmap_bottom (fdom \<rho> \<union> fst ` set ((x, e) # removeAll (x, e) \<Gamma>)))
-                   (\<Lambda> \<rho>'a. fmap_update \<rho>
-                            (fmap_restr (fst ` set (removeAll (x, e) \<Gamma>)) (\<lbrace>removeAll (x, e) \<Gamma>\<rbrace>\<rho>'a)(x f\<mapsto> \<lbrakk> e \<rbrakk>\<^bsub>\<lbrace>removeAll (x, e) \<Gamma>\<rbrace>\<rho>'a\<^esub>)))"
+  have "... = fix_on ?S
+     (\<lambda>\<rho>'. (\<lbrace>removeAll (x, e) \<Gamma>\<rbrace>\<rho>') \<squnion>
+            (fmap_bottom (fdom \<rho> \<union> fst ` set ((x, e) # removeAll (x, e) \<Gamma>))(x f\<mapsto> \<lbrakk> e \<rbrakk>\<^bsub>\<rho>'\<^esub>) \<squnion>
+             fmap_expand \<rho> (fdom \<rho> \<union> fst ` set ((x, e) # removeAll (x, e) \<Gamma>))))"                           
+    by (rule iterative_HSem[OF cond xnot1])
+  also
+  have "... = fix_on ?S
+     (\<lambda>\<rho>'. (\<lbrace>removeAll (x, e) \<Gamma>\<rbrace>\<rho>') \<squnion>
+            (fmap_bottom (fdom \<rho> \<union> fst ` set ((x, e) # removeAll (x, e) \<Gamma>))(x f\<mapsto> \<lbrakk> e \<rbrakk>\<^bsub>\<lbrace>removeAll (x, e) \<Gamma>\<rbrace>\<rho>'\<^esub>) \<squnion>
+             fmap_expand \<rho> (fdom \<rho> \<union> fst ` set ((x, e) # removeAll (x, e) \<Gamma>))))"                           
     sorry also (* Unfolding a bit under the fixed point, as in 5.2.1 *)
-  have "... = fix1 (fmap_bottom (fdom \<rho> \<union> fst ` set ((x, e) # removeAll (x, e) \<Gamma>)))
-                   (\<Lambda> \<rho>'a. fmap_update \<rho>
-                            (fmap_restr (fst ` set (removeAll (x, e) \<Gamma>)) (\<lbrace>removeAll (x, e) \<Gamma>\<rbrace>\<rho>'a)(x f\<mapsto> \<lbrakk> z \<rbrakk>\<^bsub>\<lbrace>\<Delta>\<rbrace>\<rho>'a\<^esub>)))"
-    by (subst  Variable.hyps(3), rule refl) also
-  have "... \<le> fix1 (fmap_bottom (fdom \<rho> \<union> fst ` set ((x, e) # removeAll (x, e) \<Gamma>)))
-                   (\<Lambda> \<rho>'a. fmap_update \<rho>
-                            (fmap_restr (fst ` set (removeAll (x, e) \<Gamma>)) (\<lbrace>\<Delta>\<rbrace>\<rho>'a)(x f\<mapsto> \<lbrakk> z \<rbrakk>\<^bsub>\<lbrace>\<Delta>\<rbrace>\<rho>'a\<^esub>)))"
+  have "... = fix_on ?S
+     (\<lambda>\<rho>'. (\<lbrace>removeAll (x, e) \<Gamma>\<rbrace>\<rho>') \<squnion>
+            (fmap_bottom (fdom \<rho> \<union> fst ` set ((x, e) # removeAll (x, e) \<Gamma>))(x f\<mapsto> \<lbrakk> z \<rbrakk>\<^bsub>\<lbrace>\<Delta>\<rbrace>\<rho>'\<^esub>) \<squnion>
+             fmap_expand \<rho> (fdom \<rho> \<union> fst ` set ((x, e) # removeAll (x, e) \<Gamma>))))"  
+   apply (rule fix_on_cong)
+   (* fix_on_cond with bit unfolded *)
+   defer
+   (* drule for refines in jfc'' *)
+   apply (rule arg_cong[OF Variable.hyps(3)])
+   defer
+   sorry also 
+   (*    by (subst  hyps(1), rule refl) also *)
+   have "... \<le> fix_on ?S
+     (\<lambda>\<rho>'. (\<lbrace>\<Delta>\<rbrace>\<rho>') \<squnion>
+            (fmap_bottom (fdom \<rho> \<union> fst ` set ((x, e) # removeAll (x, e) \<Gamma>))(x f\<mapsto> \<lbrakk> z \<rbrakk>\<^bsub>\<lbrace>\<Delta>\<rbrace>\<rho>'\<^esub>) \<squnion>
+             fmap_expand \<rho> (fdom \<rho> \<union> fst ` set ((x, e) # removeAll (x, e) \<Gamma>))))"
     using Variable.hyps(4)
     (* \<le> and fix1 *)
     sorry also
-  have "... \<le> fix1 (fmap_bottom (fdom \<rho> \<union> fst ` set ((x, z) # \<Delta>) ))
-                   (\<Lambda> \<rho>'a. fmap_update \<rho>
-                            (fmap_restr (fst ` set \<Delta>) (\<lbrace>\<Delta>\<rbrace>\<rho>'a)(x f\<mapsto> \<lbrakk> z \<rbrakk>\<^bsub>\<lbrace>\<Delta>\<rbrace>\<rho>'a\<^esub>)))"
-    (* Extending the domain *)
+  have "... = fix_on ?S2
+     (\<lambda>\<rho>'. (\<lbrace>\<Delta>\<rbrace>\<rho>') \<squnion>
+            (fmap_bottom (fdom \<rho> \<union> fst ` set ((x, z) # \<Delta>))(x f\<mapsto> \<lbrakk> z \<rbrakk>\<^bsub>\<lbrace>\<Delta>\<rbrace>\<rho>'\<^esub>) \<squnion>
+             fmap_expand \<rho> (fdom \<rho> \<union> fst ` set ((x, z) # \<Delta>))))"
+    (* fdoms anpassen *)
     sorry also
-  have "... \<le> fix1 (fmap_bottom (fdom \<rho> \<union> fst ` set ((x, z) # \<Delta>) ))
-                   (\<Lambda> \<rho>'a. fmap_update \<rho>
-                            (fmap_restr (fst ` set \<Delta>) (\<lbrace>\<Delta>\<rbrace>\<rho>'a)(x f\<mapsto> \<lbrakk> z \<rbrakk>\<^bsub>\<rho>'a\<^esub>)))"
+  have "... = fix_on ?S2
+     (\<lambda>\<rho>'. (\<lbrace>\<Delta>\<rbrace>\<rho>') \<squnion>
+            (fmap_bottom (fdom \<rho> \<union> fst ` set ((x, z) # \<Delta>))(x f\<mapsto> \<lbrakk> z \<rbrakk>\<^bsub>\<rho>'\<^esub>) \<squnion>
+             fmap_expand \<rho> (fdom \<rho> \<union> fst ` set ((x, z) # \<Delta>))))"
     (* Again 5.2.1 *)
     sorry also
   have  "... = \<lbrace>(x, z) # \<Delta>\<rbrace>\<rho>"
-    by (rule iterative_HSem[OF xnot2,symmetric])
+    by (rule iterative_HSem[OF cond2  xnot2,symmetric])
   finally show part2: ?case.
+
+  case 3 show ?case sorry
 
   case 1
   have "\<lbrakk> Var x \<rbrakk>\<^bsub>\<lbrace>\<Gamma>\<rbrace>\<rho>\<^esub> = the (lookup (\<lbrace>\<Gamma>\<rbrace>\<rho>) x)" by simp also
@@ -98,29 +149,43 @@ case (Variable x e \<Gamma> L \<Delta> z \<rho>)
     using part2 (* Definition of \<le> and existence of x in \<Gamma> *)
     sorry also
   have "... = \<lbrakk> z \<rbrakk>\<^bsub>\<lbrace>(x,z) # \<Delta>\<rbrace>\<rho>\<^esub>"
-    by (subst HSem_unroll, auto)
+    apply (subst HSem_unroll[OF cond2])
+    apply (subst the_lookup_join[OF rho_F_compat_jfc''[OF cond2 HSem_there[OF cond2]]])
+    apply auto
+    apply (rule larger_is_join)
+    apply (cases "x \<in> fdom \<rho>")
+    apply (rule below_trans[OF refinesD'[OF  `refines ((x, z) # \<Delta>) \<rho>`, simplified]])
+    apply auto[2]
+    apply (rule cont2monofunE[OF ESem_cont HSem_refines[OF cond2, simplified]])
+    apply simp
+    done
   finally show ?case.
 next
 
 case (Let as \<Gamma> L body \<Delta> z \<rho>)
+  note `set (bn as) \<sharp>* L` (* Does this help? fdom \<rho> = L? *)
   have "set (bn as) \<sharp>* \<rho>" sorry (* Problem: How to achieve this? *)
   with `set (bn as) \<sharp>* \<Gamma>`
-  have "set (bn as) \<sharp>* (\<lbrace>\<Gamma>\<rbrace>\<rho>)" sorry  
+  have "set (bn as) \<sharp>* (\<lbrace>\<Gamma>\<rbrace>\<rho>)" sorry
+
+  have "refines (asToHeap as @ \<Gamma>) \<rho>" sorry
+ 
+  note hyps = Let.hyps(4-6)[OF `refines (asToHeap as @ \<Gamma>) \<rho>`]
 
   case 1
   have "\<lbrakk> Let as body \<rbrakk>\<^bsub>\<lbrace>\<Gamma>\<rbrace>\<rho>\<^esub> = \<lbrakk> body \<rbrakk>\<^bsub>\<lbrace>asToHeap as\<rbrace>\<lbrace>\<Gamma>\<rbrace>\<rho>\<^esub>"
     by (rule Esem_simps4[OF `set (bn as) \<sharp>* (\<lbrace>\<Gamma>\<rbrace>\<rho>)`]) also
   have "... = \<lbrakk> body \<rbrakk>\<^bsub>\<lbrace>asToHeap as @ \<Gamma>\<rbrace>\<rho>\<^esub>" sorry also
-  have "... = \<lbrakk> z \<rbrakk>\<^bsub>\<lbrace>\<Delta>\<rbrace>\<rho>\<^esub>" by fact
+  have "... = \<lbrakk> z \<rbrakk>\<^bsub>\<lbrace>\<Delta>\<rbrace>\<rho>\<^esub>" by (rule hyps)
   finally show ?case .
 
   case 2
   have "\<lbrace>\<Gamma>\<rbrace>\<rho> \<le> \<lbrace>asToHeap as @ \<Gamma>\<rbrace>\<rho>" sorry also
-  have "... \<le> \<lbrace>\<Delta>\<rbrace>\<rho>" by fact
+  have "... \<le> \<lbrace>\<Delta>\<rbrace>\<rho>" by (rule hyps)
   finally show ?case .
 
+  case 3 show ?case by (rule hyps)
 qed
 
 end
-
 
